alt def of alpha eq

vtr/coq/lib/Semantics/PolyTyp.v
@@ -40,15 +40,15 @@ Proof.
   dispatch_eqdec; inv H; eauto.
 Qed.
 
-Definition alpha
-           '(∀ XS, x : poly)
-           '(∀ YS, y : poly) : Prop :=
-  x = ~[ uniques YS ⟼  map TVar (uniques XS) ]~ † y.
+Reserved Notation "p1 ≂ p2" (at level 70, no associativity).
 
-Notation "p1 ≂ p2"
-  := (alpha p1 p2)
-       (at level 70, no associativity) : type_scope.
+Inductive alpha (p : poly) : poly -> Prop :=
+| alpha_eq YS :
+  Forall (fun Y => Y ∉ ptvars p) YS ->
+  p ≂ ∀ YS, ~[pvars p ⟼  map TVar YS]~ † ptyp p
+where "p1 ≂ p2" := (alpha p1 p2) : type_scope.
 
+(*
 Section AlphaExamples.
   Local Hint Unfold alpha : core.
   Local Hint Unfold combine_to_env : core.
@@ -98,10 +98,9 @@ Section AlphaExamples.
     figure.
   Qed.
 End AlphaExamples.
+*)
 
 Section Alpha.
-  Local Hint Unfold alpha : core.
-    
   Lemma tvars_sub_tvar_same : forall TS T,
     match ~[ TS ⟼ map TVar TS ]~ T with
     | Some τ => τ
@@ -121,184 +120,55 @@ Section Alpha.
       intro TS; simpl; auto; f_equal; auto.
   Qed.
 
-  Local Hint Resolve tvars_tsub_same : core.
+  (* Local Hint Resolve tvars_tsub_same : core. *)
   Local Hint Unfold Reflexive : core.
+  Local Hint Constructors alpha : core.
+
+  Lemma ptvars_same_Forall : forall XS x,
+      Forall (fun Y : nat => Y ∉ ptvars (∀ XS, x)) XS.
+  Proof.
+    simpl; intro XS; induction XS as [| X XS IHXS];
+      intro x; simpl in *; auto.
+    constructor; simpl.
+    - pose proof difference_Difference (tvars x) (X :: XS) as Hd.
+      unfold Difference in Hd.
+      intros H. firstorder.
+    - rewrite Forall_forall.
+      intros n HnXS Hin.
+      specialize IHXS with x.
+      rewrite Forall_forall in IHXS.
+      specialize IHXS with n.
+      apply IHXS in HnXS.
+      rewrite remove_diff_cons in Hin.
+      apply remove_sound in Hin. contradiction.
+  Qed.
+
+  Local Hint Resolve ptvars_same_Forall : core.
   
   Lemma alpha_reflexive : Reflexive alpha.
   Proof.
-    autounfold with core; intros [XS x]; auto.
+    autounfold with core; intros [XS x].
+    rewrite <- tvars_tsub_same with (TS := XS) at 2.
+    constructor; auto.
   Qed.
 
-  Lemma tvars_tsub_tvar_involutive : forall XS YS T,
-      NoDup XS -> NoDup YS ->
-      ~[XS ⟼  map TVar YS]~
-       † match ~[YS ⟼  map TVar XS]~ T with
-         | Some τ => τ
-         | None => T
-         end = T.
-  Proof.
-    intros XS YS T Hndx Hndy.
-    destruct (~[YS ⟼  map TVar XS]~ T)
-      as [t |] eqn:Heqt;
-      try apply combine_binds_only_tvar in Heqt as HOT;
-      try destruct HOT as [Z HZ]; subst; simpl.
-    - destruct (~[XS ⟼  map TVar YS]~ Z)
-        as [t |] eqn:Heqt';
-        try apply combine_binds_only_tvar in Heqt' as HOT;
-        try destruct HOT as [W HW]; subst; simpl.
-      + rewrite combine_to_env_lookup in Heqt.
-        rewrite combine_to_env_lookup in Heqt'.
-        apply lookup_in in Heqt  as HT.
-        apply lookup_in in Heqt' as HZ.
-        rewrite combine_map_r in HT, HZ.
-        rewrite in_map_iff in HT, HZ.
-        destruct HT as ((x1 & x2) & H1 & HYX);
-          destruct HZ as ((x3 & x4) & H2 & HXY);
-          inv H1; inv H2.
-        apply in_combine_flip in HYX.
-        eauto using NoDup_pair_eq_r.
-      + exfalso.
-        rewrite combine_to_env_lookup in Heqt, Heqt'.
-        apply lookup_in in Heqt as HT.
-        apply lookup_not_in with (v:=TVar T) in Heqt' as HZ.
-        rewrite combine_map_r in HT, HZ.
-        rewrite in_map_iff in HT, HZ.
-        destruct HT as ((x1 & x2) & Huv & HYXS); inv Huv.
-        apply in_combine_flip in HYXS. firstorder.
-    - destruct (~[XS ⟼  map TVar YS]~ T)
-        as [t |] eqn:Heqt';
-        try apply combine_binds_only_tvar in Heqt' as HOT;
-        try destruct HOT as [W HW]; subst; simpl; auto.
-      (* apply combine_to_env_some in Heqt'
-        as (XS1 & XS2 & YS1 & YS2 & HC & HTXS1). *)
-      rewrite combine_to_env_lookup in Heqt, Heqt'.
-      pose proof lookup_not_in _ _ Heqt T as HT.
-      apply lookup_in in Heqt' as HW.
-      rewrite combine_map_r in HT, HW.
-      rewrite in_map_iff in HT, HW.
-      destruct HW as ((x1 & x2) & Huv & HYXS); inv Huv.
-      apply nexists_forall_not with (x:=(T, T)) in HT.
-      apply Decidable.not_and in HT; firstorder.
-      apply not_in_combine in H.
-      apply in_combine_nth_error in HYXS as (n & HXS & HYS).
-      apply nth_error_In in HXS as HXSin;
-        apply nth_error_In in HYS as HYSin.
-      destruct H as [Htyxs | [Htyxs | [Htyxs | Hmn]]];
-        try destruct Htyxs as [Htxs Htys];
-        try destruct Hmn as (p & q & Hpq & Hp & Hq);
-        try contradiction.
-      + admit.
-  Abort.
-      
-  Lemma tvars_tsub_involutive : forall t XS YS,
-      NoDup XS -> NoDup YS ->
-      ~[ XS ⟼ map TVar YS ]~ † ~[ YS ⟼ map TVar XS ]~ † t = t.
-  Proof.
-    intro t; induction t as [| | t1 IHt1 t2 IHt2 | T];
-      intros XS YS Hndx Hndy; try (simpl; auto; assumption).
-    - simpl; rewrite IHt1, IHt2; auto.
-    - rewrite tsub_assoc.
-      unfold "‡"; simpl.
-      (* let X ≠ Y.
-         ∴ (X ↦ Y) † (Y ↦ X) † X = (X ↦ Y) X = Y ≠ X.
-         ∀ [X], X ≂ ∀ [Y], Y ↔ X = (Y ↦ X) † Y = X
-         ∴ ∀ [X], X ≂ ∀ [Y], Y.
-         ∀ [Y], Y ≂ ∀ [X], X ↔ Y = (X ↦ Y) † X = Y
-         ∴ ∀ [Y], Y ≂ ∀ [X], X.
-       *)
-  Abort.
-  
   Local Hint Unfold Symmetric : core.
 
   Lemma alpha_symmetric : Symmetric alpha.
   Proof.
-    autounfold with *; intros [XS x] [YS y] H.
-    generalize dependent YS;
-      generalize dependent XS;
-      generalize dependent y.
-    induction x as [| | x1 IHx1 x2 IHx2 | X];
-      intros [| | y1 y2 | Y] XS YS Hxy;
-      try (simpl in *; try discriminate; auto; assumption).
-    - simpl in *.
-      destruct
-        (~[ uniques YS ⟼ map TVar (uniques XS) ]~ Y)
-        as [z |] eqn:Hz;
-        try apply combine_binds_only_tvar in Hz as [Z HZ];
-        subst; try discriminate.
-    - simpl in *.
-      destruct
-        (~[ uniques YS ⟼ map TVar (uniques XS) ]~ Y)
-        as [z |] eqn:Hz;
-        try apply combine_binds_only_tvar in Hz as [Z HZ];
-        subst; try discriminate.
-    - simpl in *.
-      injection Hxy as Hx1 Hx2.
-      apply IHx1 in Hx1. apply IHx2 in Hx2.
-      subst; reflexivity.
-    - simpl in *.
-      destruct
-        (~[ uniques YS ⟼ map TVar (uniques XS) ]~ Y)
-        as [z |] eqn:Hz;
-        try apply combine_binds_only_tvar in Hz as [Z HZ];
-        subst; try discriminate.
-    - (* Either:
-         1. [Y] is bound in [YS],
-            & if [length XS <= length YS]
-            the substitution is bijective;
-            thus the goal is satisfied.
-         2. [Y] is not bound in [YS],
-            suggesting [X = Y],
-            & [Y] is free in [∀ YS, y].
-            a. [Y] is not bound in XS; thus trivial.
-            b. [Y] is bound in [XS],
-               & if [length YS <= length XS]
-               & [Y] is not free in [∀ XS, x].
-               then trouble starts, b/c
-               [Y] will be mapped to some [W] in [YS].
-               We know that [Y <> W] b/c
-               [In W YS /\ ~ In Y YS]. *)
-      (* An example of the problem:
-         Consider [x = ∀ [X], X], [y = ∀ [Y], X].
-         [X = (Y ↦ X) † X = X] whether or not [X = Y].
-         ∴ by my def [∀ [X], X] ≂ ∀ [Y], X].
-         This is bad because [x] is not alpha equivalent to [y].
-         [X = (X ↦ Y) † X = Y] only makes sense if [X = Y].
-         Thus my definition [≂] is flawed. *)
-      simpl in *.
-      destruct
-        (~[ uniques YS ⟼ map TVar (uniques XS) ]~ Y)
-        as [z |] eqn:Hz;
-        try apply combine_binds_only_tvar in Hz as Hz';
-        try destruct Hz' as [Z HZ].
-      + subst. inv Hxy.
-        destruct
-          (~[ uniques XS ⟼ map TVar (uniques YS) ]~ Z)
-          as [w |] eqn:Hw;
-          try apply combine_binds_only_tvar in Hw as Hw';
-          try destruct Hw' as [W HW]; subst.
-        * (* provable. *) admit.
-        * (* contradiction. *) admit.
-      + inv Hxy.
-        destruct
-          (~[ uniques XS ⟼ map TVar (uniques YS) ]~ Y)
-          as [w |] eqn:Hw;
-          try apply combine_binds_only_tvar in Hw as Hw';
-          try destruct Hw' as [W HW];
-          subst; auto.
-        (* stuck in the same way:
-           provably [Y <> W];
-           but the goal is [Y = W]. *)
-      (*
-    rewrite H.
-    enough (XS = [0]).
-    enough (YS = [1]).
-    enough (x = 1).
-    enough (y = 0).
-    { subst.
-      unfold uniques, remove,
-      combine_to_env, combine,
-      to_env, map, fold_right, uncurry in *.
-      simpl in *. *)
+    autounfold with *; intros [XS x] [YS y] H; inv H.
+    rename H1 into H.
+    pose proof tvars_tsub_same x YS as Hy.
+    pose proof alpha_eq
+         (∀ YS, ~[ XS ⟼ map TVar YS ]~ † x) XS as Ha; simpl in Ha.
+  Abort.
+
+  Local Hint Unfold Transitive : core.
+  
+  Lemma alpha_transitive : Transitive alpha.
+  Proof.
+    autounfold with *; intros [XS x] [YS y] [ZS z] Hxy Hyz.
+    inv Hxy; inv Hyz.
   Abort.
 End Alpha.
 
